SQC 1:
\left| q_i \right\rangle = R_y(\theta_i) H \left| 0 \right\rangle


SQC 2:
H \left| 0 \right\rangle = \frac{\left| 0 \right\rangle + \left| 1 \right\rangle}{\sqrt{2}}

SQC 3:
R_y(\theta_i) \frac{\left| 0 \right\rangle + \left| 1 \right\rangle}{\sqrt{2}} = \cos\left(\frac{\theta_i}{2}\right) \frac{\left| 0 \right\rangle + \left| 1 \right\rangle}{\sqrt{2}} + \sin\left(\frac{\theta_i}{2}\right) \frac{\left| 1 \right\rangle - \left| 0 \right\rangle}{\sqrt{2}}


EQC 1:
\left| q_i \right\rangle = R_y(\theta_i) H \left| 0 \right\rangle

EQC 2:
\left| q_j \right\rangle = R_y(\theta_j) H \left| 0 \right\rangle

EQC 3:
\left| q_i, q_j \right\rangle = \text{CNOT} \left( R_y(\theta_i) H \left| 0 \right\rangle \otimes R_y(\theta_j) H \left| 0 \right\rangle \right)


AQC 1:


